src/HOL/Library/Code_Abstract_Nat.thy
@@ -113,4 +113,17 @@ in
 end
 \<close>
 
+
+subsection \<open>One candidate which needs special treatment\<close>
+
+lemma take_bit_num_code [code]:
+  \<open>take_bit_num n Num.One =
+    (case n of 0 \<Rightarrow> None | Suc n \<Rightarrow> Some Num.One)\<close>
+  \<open>take_bit_num n (Num.Bit0 m) =
+    (case n of 0 \<Rightarrow> None | Suc n \<Rightarrow> (case take_bit_num n m of None \<Rightarrow> None | Some q \<Rightarrow> Some (Num.Bit0 q)))\<close>
+  \<open>take_bit_num n (Num.Bit1 m) =
+    (case n of 0 \<Rightarrow> None | Suc n \<Rightarrow> Some (case take_bit_num n m of None \<Rightarrow> Num.One | Some q \<Rightarrow> Num.Bit1 q))\<close>
+    apply (cases n; simp)+
+  done
+
 end
